Beautiful Proofs !

theories/RTL.v
@@ -52,7 +52,6 @@ Record function := {
     fn_regs: list reg;
     fn_entrypoint : node;
     fn_code : code;
-
     fn_regs_no_dup : NoDup fn_regs;
 }.
 
@@ -60,3 +59,58 @@ Definition program := list function.
 
 Definition find_fun (P: program) (s: ident) : option function :=
   List.find (fun f => (fn_name f =? s)%string) P.
+
+(* [regmap] is a mapping from registers to a value *)
+Definition regmap : Type := gmap reg val.
+
+(* [memory] is a mapping from location to a value *)
+Definition memory : Type := gmap loc val.
+
+Definition val_to_loc (v: val) : option loc :=
+  if (v >=? 1)%Z
+  then Some (Z.to_pos v)
+  else None.
+
+Definition get_reg (r: reg) (ρ: regmap) : val :=
+  match ρ !! r with
+  | Some v => v
+  | None => 0%Z (* Dummy val *)
+  end.
+
+Definition get_regs (l: list reg) (ρ: regmap) : list val :=
+  map (fun r => get_reg r ρ) l.
+
+Definition set_reg (r: reg) (v: val) (ρ: regmap) : regmap := <[r := v]>ρ.
+
+Definition get_at (addr: val) (m: memory) : option val :=
+  match val_to_loc addr with
+  | Some loc => m !! loc
+  | None => None
+  end.
+
+Definition update_at (addr: val) (f: val -> val) (m: memory) : option memory
+  := match val_to_loc addr with
+     | Some loc =>
+         match m !! loc with
+         | Some old => Some (<[loc := f old]>m)
+         | None => None
+         end
+     | None => None
+     end.
+
+Definition set_at (addr: val) (v: val) (m: memory) : option memory :=
+  update_at addr (fun _ => v) m.
+
+(* Assert that instruction at [pc] in function [f] is [i] *)
+Notation "f '@' pc 'is' i" :=
+  ((fn_code f)!!pc = Some i) (at level 60, no associativity).
+
+Definition eval_op (op: op) (args: list val) : option val :=
+  match op, args with
+  | Add, [v1; v2] => Some (v1 + v2)%Z
+  | Sub, [v1; v2] => Some (v1 - v2)%Z
+  | Mul, [v1; v2] => Some (v1 * v2)%Z
+  | Move, [v] => Some v
+  | LoadI v, [] => Some v
+  | _, _ => None
+  end.
