theories/Semantics.v
@@ -8,67 +8,13 @@ From stdpp Require Import relations.
 From stdpp Require Import tactics.
 
 From RSL Require Import RTL.
+From RSL Require Import Logic.
 From RSL Require Import Notations.
 
 Import RTLNotations.
 Import ListNotations.
 
 (* Set Mangle Names. *)
-
-(* [regmap] is a mapping from registers to a value *)
-Definition regmap : Type := gmap reg val.
-
-(* [memory] is a mapping from location to a value *)
-Definition memory : Type := gmap loc val.
-
-Definition val_to_loc (v: val) : option loc :=
-  if (v >=? 1)%Z
-  then Some (Z.to_pos v)
-  else None.
-
-Definition get_reg (r: reg) (ρ: regmap) : val :=
-  match ρ !! r with
-  | Some v => v
-  | None => 0%Z (* Dummy val *)
-  end.
-
-Definition get_regs (l: list reg) (ρ: regmap) : list val :=
-  map (fun r => get_reg r ρ) l.
-
-Definition set_reg (r: reg) (v: val) (ρ: regmap) : regmap := <[r := v]>ρ.
-
-Definition get_at (addr: val) (m: memory) : option val :=
-  match val_to_loc addr with
-  | Some loc => m !! loc
-  | None => None
-  end.
-
-Definition update_at (addr: val) (f: val -> val) (m: memory) : option memory
-  := match val_to_loc addr with
-     | Some loc =>
-         match m !! loc with
-         | Some old => Some (<[loc := f old]>m)
-         | None => None
-         end
-     | None => None
-     end.
-
-Definition set_at (addr: val) (v: val) (m: memory) : option memory :=
-  update_at addr (fun _ => v) m.
-
-(* Assert that instruction at [pc] in function [f] is [i] *)
-Notation "f '@' pc 'is' i" :=
-  ((fn_code f)!!pc = Some i) (at level 60, no associativity).
-
-Definition eval_op (op: op) (args: list val) : option val :=
-  match op, args with
-  | Add, [v1; v2] => Some (v1 + v2)%Z
-  | Sub, [v1; v2] => Some (v1 - v2)%Z
-  | Mul, [v1; v2] => Some (v1 * v2)%Z
-  | Move, [v] => Some v
-  | LoadI v, [] => Some v
-  | _, _ => None
-  end.
 
 Fixpoint init_regs (vl: list val) (rl: list reg) : regmap :=
   match rl, vl with
@@ -100,65 +46,65 @@ Inductive pcstate : Type :=
 
 Definition state : Type := list stackframe * pcstate * memory.
 
-Reserved Notation "P '|-' s '->>' t" (at level 60, right associativity).
+Reserved Notation "P '⊨' s '->>' t" (at level 60, right associativity).
 
 Inductive step (P: program) : state -> state -> Prop :=
 | exec_Inop: forall σ m ρ f pc pc',
   f@pc is <{ nop -> pc' }> ->
-  P |- (σ, State f pc ρ, m) ->> (σ, State f pc' ρ, m)
+  P ⊨ (σ, State f pc ρ, m) ->> (σ, State f pc' ρ, m)
 
 | exec_Iret: forall σ m ρ f pc r v,
   f@pc is <{ ret r }> ->
   get_reg r ρ = v ->
-  P |- (σ, State f pc ρ, m) ->> (σ, ReturnState v, m)
+  P ⊨ (σ, State f pc ρ, m) ->> (σ, ReturnState v, m)
 
 | exec_Iop: forall σ m ρ f pc op args dst pc' ρ' v,
   f@pc is <{ dst := @op args -> pc' }> ->
   eval_op op (get_regs args ρ) = Some v ->
   set_reg dst v ρ = ρ' ->
-  P |- (σ, State f pc ρ, m) ->> (σ, State f pc' ρ', m)
+  P ⊨ (σ, State f pc ρ, m) ->> (σ, State f pc' ρ', m)
 
 | exec_Iload: forall σ m ρ f pc dst src pc' ρ' addr v,
   f@pc is <{ dst := !src -> pc' }> ->
   get_reg src ρ = addr ->
   get_at addr m = Some v ->
   set_reg dst v ρ = ρ' ->
-  P |- (σ, State f pc ρ, m) ->> (σ, State f pc' ρ', m)
+  P ⊨ (σ, State f pc ρ, m) ->> (σ, State f pc' ρ', m)
 
 | exec_Istore: forall σ m ρ f pc dst src pc' m' addr v,
   f@pc is <{ !dst := src -> pc' }> ->
   get_reg dst ρ = addr ->
   get_reg src ρ = v ->
   set_at addr v m = Some m' ->
-  P |- (σ, State f pc ρ, m) ->> (σ, State f pc' ρ, m')
+  P ⊨ (σ, State f pc ρ, m) ->> (σ, State f pc' ρ, m')
 
 | exec_Icond: forall  σ m ρ f pc cond ifso ifnot v pc',
   f@pc is <{ if cond then goto ifso else goto ifnot }> ->
   get_reg cond ρ = v ->
   pc' = (if Z.eqb v 0 then ifso else ifnot) ->
-  P |- (σ, State f pc ρ, m) ->> (σ, State f pc' ρ, m)
+  P ⊨ (σ, State f pc ρ, m) ->> (σ, State f pc' ρ, m)
 
 | exec_Icall: forall σ m ρ f pc dst sig args pc' σ' fn,
   f@pc is <{ dst := @call sig args -> pc' }> ->
   find_fun P sig = Some fn ->
   Stackframe dst f pc' ρ :: σ = σ' ->
-  P |- (σ, State f pc ρ, m) ->> (σ', CallState fn (get_regs args ρ), m)
+  P ⊨ (σ, State f pc ρ, m) ->> (σ', CallState fn (get_regs args ρ), m)
 
 | exec_function: forall σ m ρ f args,
   length args = length (fn_regs f) ->
   init_regs args (fn_regs f) = ρ ->
-  P |- (σ, CallState f args, m) ->> (σ, State f (fn_entrypoint f) ρ, m)
+  P ⊨ (σ, CallState f args, m) ->> (σ, State f (fn_entrypoint f) ρ, m)
 
 | exec_return: forall σ m ρ f pc dst v ρ',
   set_reg dst v ρ = ρ' ->
-  P |- (Stackframe dst f pc ρ :: σ, ReturnState v, m) ->> (σ, State f pc ρ', m)
+  P ⊨ (Stackframe dst f pc ρ :: σ, ReturnState v, m) ->> (σ, State f pc ρ', m)
 
-where "P '|-' s '->>' t" := (step P s t).
+where "P '⊨' s '->>' t" := (step P s t).
 
-Notation "P '|-' s '->>*' t" :=
+Notation "P '⊨' s '->>*' t" :=
   (rtc (step P) s t)  (at level 60, right associativity).
 
-Notation "P '|-' s '-{' n '}>' t" :=
+Notation "P '⊨' s '-{' n '}>' t" :=
   (nsteps (step P) n s t)  (at level 60, right associativity).
 
 Lemma nsteps_inv_l {A : Type} {R : relation A} :
@@ -166,7 +112,7 @@ Lemma nsteps_inv_l {A : Type} {R : relation A} :
 Proof. intros n x z H; inv H; eexists; eauto. Qed.
 
 Lemma ret_no_step P : ∀ v m t,
-  P |- ([], ReturnState v, m) ->>* t ->
+  P ⊨ ([], ReturnState v, m) ->>* t ->
   t = ([], ReturnState v, m).
 Proof.
   intros v m t H.
@@ -176,7 +122,7 @@ Proof.
 Qed.
 
 Lemma ret_no_nsteps P : ∀ n v m t,
-  P |- ([], ReturnState v, m) -{n}> t ->
+  P ⊨ ([], ReturnState v, m) -{n}> t ->
   t = ([], ReturnState v, m) ∧ n = 0.
 Proof.
   intros [] v m t H.
@@ -186,15 +132,15 @@ Proof.
 Qed.
 
 Lemma lift_step P : ∀ σ s m σ' t m' Σ,
-  P |- (σ, s, m) ->> (σ', t, m') ->
-  P |- (σ ++ Σ, s, m) ->> (σ' ++ Σ, t, m').
+  P ⊨ (σ, s, m) ->> (σ', t, m') ->
+  P ⊨ (σ ++ Σ, s, m) ->> (σ' ++ Σ, t, m').
 Proof.
   intros ? ? ? ? ? ? ? H; inv H; econstructor; now eauto.
 Qed.
 
 Lemma unlift_step P : ∀ σ s m σ' t m' Σ,
-  P |- (σ ++ Σ, s, m) ->> (σ' ++ Σ, t, m') ->
-  P |- (σ, s, m) ->> (σ', t, m').
+  P ⊨ (σ ++ Σ, s, m) ->> (σ' ++ Σ, t, m') ->
+  P ⊨ (σ, s, m) ->> (σ', t, m').
 Proof.
   intros ? ? ? ? ? ? ? H; inv H;
     rewrite ? app_comm_cons in *;
@@ -203,13 +149,13 @@ Proof.
 Qed.
 
 Theorem step_callstack P : ∀ σ s m σ' t m' Σ,
-  P |- (σ, s, m) ->> (σ', t, m') <->
-  P |- (σ ++ Σ, s, m) ->> (σ' ++ Σ, t, m').
+  P ⊨ (σ, s, m) ->> (σ', t, m') <->
+  P ⊨ (σ ++ Σ, s, m) ->> (σ' ++ Σ, t, m').
 Proof. split. 1: apply lift_step. apply unlift_step. Qed.
 
 Theorem lift_steps P : ∀ σ s m σ' t m' Σ,
-  P |- (σ, s, m) ->>* (σ', t, m') ->
-  P |- (σ ++ Σ, s, m) ->>* (σ' ++ Σ, t, m').
+  P ⊨ (σ, s, m) ->>* (σ', t, m') ->
+  P ⊨ (σ ++ Σ, s, m) ->>* (σ' ++ Σ, t, m').
 Proof.
   intros σ s m σ' t m' Σ Hrtc.
   remember (σ, s, m) as x eqn:Hx.
@@ -224,15 +170,15 @@ Proof.
 Qed.
 
 Lemma unfold_call P fn : ∀ n res f pc ρ args m σ t m',
-  P |- ([Stackframe res f pc ρ], CallState fn args, m) -{n}> (σ, t, m') ->
+  P ⊨ ([Stackframe res f pc ρ], CallState fn args, m) -{n}> (σ, t, m') ->
   (∃ σ',
       σ = σ' ++ [Stackframe res f pc ρ]
-      ∧ P |- ([], CallState fn args, m) -{n}> (σ', t, m'))
+      ∧ P ⊨ ([], CallState fn args, m) -{n}> (σ', t, m'))
   ∨
     (∃ m1 m2 v m'',
         n = 1 + m1 + m2
-        ∧ P |- ([], CallState fn args, m) -{m1}> ([], ReturnState v, m'')
-        ∧ P |- ([], State f pc (set_reg res v ρ), m'') -{m2}> (σ, t, m')
+        ∧ P ⊨ ([], CallState fn args, m) -{m1}> ([], ReturnState v, m'')
+        ∧ P ⊨ ([], State f pc (set_reg res v ρ), m'') -{m2}> (σ, t, m')
     ).
 Proof.
   intros n.
@@ -309,6 +255,9 @@ Tactic Notation "simpl_reg" "by" tactic3(tac) :=
     | |- context[get_reg _ (set_reg _ _ _)] =>
         (rewrite get_reg_set_reg_neq by tac)
         || (rewrite get_reg_set_reg_eq by tac)
+    | H: get_reg ?r ?rho = _ |- context[get_reg ?r ?rho] =>
+        repeat rewrite H
     end.
 
-Tactic Notation "simpl_reg" := simpl_reg by (f_equal; lia).
+Tactic Notation "simpl_reg" :=
+  simpl_reg by repeat (f_equal || lia || unfold_Prop || split).
