theories/Logic.v
@@ -1,40 +1,50 @@
 From Stdlib Require Import Utf8.
 
 From RSL Require Import RTL.
-From RSL Require Import Semantics.
 
 (* Set Mangle Names. *)
-
-Definition oProp : Type := memory -> nat -> Prop.
-Definition sProp : Type := regmap -> oProp.
 
 Definition postcondition : Type := val -> memory -> Prop.
 Definition precondition : Type := list val -> memory -> Prop.
 
-Definition lift_oProp (P : oProp) : sProp :=  fun _ => P.
-Coercion lift_oProp : oProp >-> sProp.
-
-Class Logic (L: Type) :=
-  {
-    logic_and : L -> L -> L;
-    logic_or  : L -> L -> L;
-    logic_impl : L -> L -> L;
-    logic_not : L -> L;
-    logic_exists {X: Type}: (X -> L) -> L;
-    logic_forall {X: Type}: (X -> L) -> L;
-
-    logic_empty_entails : L -> Prop;
-    logic_pure : Prop -> L;
-    logic_memory_pure : (memory -> Prop) -> L;
-    logic_later : L -> L;
-    logic_always : L -> L;
-    logic_memory_entails : L -> L;
-  }.
+Definition logic : Type := regmap -> memory -> nat -> Prop.
 
 Declare Scope logic_scope.
 Delimit Scope logic_scope with logic.
-Bind Scope logic_scope with oProp.
-Bind Scope logic_scope with sProp.
+Bind Scope logic_scope with logic.
+
+Definition logic_and (P Q: logic) : logic :=
+  fun ρ m n => P ρ m n ∧ Q ρ m n.
+Definition logic_or (P Q: logic) : logic :=
+  fun ρ m n => P ρ m n ∨ Q ρ m n.
+Definition logic_impl (P Q: logic) : logic :=
+  fun ρ m n => P ρ m n -> Q ρ m n.
+Definition logic_not (P: logic) : logic :=
+  fun ρ m n => ~ P ρ m n.
+Definition logic_exists {X: Type} (f: X -> logic) : logic :=
+  fun ρ m n => ∃ x, f x ρ m n.
+Definition logic_forall {X: Type} (f: X -> logic) : logic :=
+  fun ρ m n => ∀ x, f x ρ m n.
+
+Definition logic_empty_entails (P: logic) : Prop :=
+  ∀ ρ m n, P ρ m n.
+Definition logic_pure (P: Prop) : logic :=
+  fun _ _ _ => P.
+Definition logic_memory_pure (P: memory -> Prop) : logic :=
+  fun _ m _ => P m.
+Definition logic_later (P: logic) : logic :=
+  fun ρ m n =>
+    match n with
+    | O => True
+    | S n => P ρ m n
+    end.
+
+Definition logic_always (P: logic) : logic :=
+  fun ρ m _ => ∀ n, P ρ m n.
+Definition logic_memory_entails (P: logic) : logic :=
+  fun ρ _ n => ∀ m, P ρ m n.
+Definition logic_register_entails (P: logic) : logic :=
+  fun _ m n => ∀ ρ, P ρ m n.
 
 Notation "P ∧ Q" :=
   (logic_and P Q) : logic_scope.
@@ -67,6 +77,9 @@ Notation "□ P" :=
 Notation "'⊢ₘ' P" :=
   (logic_memory_entails P)
     (at level 99, right associativity) : logic_scope.
+Notation "'⊢ᵨ' P" :=
+  (logic_register_entails P)
+    (at level 99, right associativity) : logic_scope.
 
 Notation "'⟨' P '⟩'" := P%logic.
 
@@ -76,101 +89,45 @@ Notation "'⟨' P '⟩'" := P%logic.
 (*   (logic_entails P%logic Q%logic) *)
 (*     (at level 99, right associativity). *)
 
-Instance oProp_logic : Logic oProp :=
-  {|
-    logic_and P Q := fun m n => P m n ∧ Q m n;
-    logic_or P Q := fun m n => P m n ∨ Q m n;
-    logic_impl P Q := fun m n => P m n -> Q m n;
-    logic_not P := fun m n => ~ P m n;
-    logic_exists X f := fun m n => ∃ x, f x m n;
-    logic_forall X f := fun m n => ∀ x, f x m n;
+Definition logic_set_mem (addr: val) (v: val) (P: logic) : logic :=
+  fun ρ m n => ∃ m', set_at addr v m = Some m' ∧ P ρ m' n.
 
-    logic_empty_entails P := ∀ m n, P m n;
-    logic_pure P := fun _ _ => P;
-    logic_memory_pure P := fun m _ => P m;
-    logic_later P :=
-      fun m n =>
-        match n with
-        | O => True
-        | S n => P m n
-        end;
+Definition logic_assert_mem (addr: val) (v: val) : logic :=
+  fun _ m _ => get_at addr m = Some v.
 
-    logic_always P := fun m _ => ∀ n, P m n;
-    logic_memory_entails P := fun _ n => ∀ m, P m n;
-  |}.
+Definition logic_set_reg (r : reg) (v : val) (P : logic) : logic :=
+  fun ρ m n => P (set_reg r v ρ) m n.
 
-Definition oProp_update (f: memory -> option memory) (P: oProp) : oProp :=
-  fun m n => ∃ m', f m = Some m' ∧ P m' n.
-
-Class oPropSetMem (L : Type) := logic_set_mem : val -> val -> L -> L.
 Notation "'⟦' addr '<-' v '⟧' P" :=
   (logic_set_mem addr v P)
     (at level 20, P at level 20, right associativity,
        format "⟦ addr <- v ⟧  P").
 
-Definition oProp_set (addr: val) (v: val) (P: oProp) : oProp :=
-  oProp_update (set_at addr v) P.
-Instance set_mem_oProp : oPropSetMem oProp := oProp_set.
-
-Instance set_mem_sProp : oPropSetMem sProp :=
-  fun addr v P ρ => oProp_set addr v (P ρ).
-
-Definition oProp_assert (addr: val) (v: val) : oProp :=
-  fun m n => get_at addr m = Some v.
 Notation "l '↦' v" :=
-  (oProp_assert l v)
+  (logic_assert_mem l v)
     (at level 70, no associativity, format "l ↦ v") : logic_scope.
 
-Instance sProp_logic : Logic sProp :=
-  {|
-    logic_and P Q := fun ρ => logic_and (P ρ) (Q ρ);
-    logic_or P Q := fun ρ => logic_or (P ρ) (Q ρ);
-    logic_impl P Q := fun ρ => logic_impl (P ρ) (Q ρ);
-    logic_not P := fun ρ => logic_not (P ρ);
-    logic_exists X f := fun ρ => logic_exists (fun x => f x ρ);
-    logic_forall X f := fun ρ => logic_forall (fun x => f x ρ);
-
-    logic_empty_entails P := ∀ ρ, logic_empty_entails (P ρ);
-    logic_pure P := fun _ => logic_pure P;
-    logic_memory_pure P := fun _ => logic_memory_pure P;
-    logic_later P := fun ρ => logic_later (P ρ);
-    logic_always P := fun ρ => logic_always (P ρ);
-    logic_memory_entails P := fun ρ => logic_memory_entails (P ρ);
-  |}.
-
-Definition sProp_set_reg (r : reg) (v : val) (P : sProp) : sProp :=
-  fun ρ => P (set_reg r v ρ).
 Notation "'⟦' dst '<-ᵣ' v '⟧' P" :=
-  (sProp_set_reg dst v P)
+  (logic_set_reg dst v P)
     (at level 20, P at level 20, right associativity,
        format "⟦ dst <-ᵣ v ⟧  P") : logic_scope.
 
-Class LogicAssertReg (R V : Type) := logic_assert_reg : R -> V -> sProp.
+Class LogicAssertReg (R V : Type) := logic_assert_reg : R -> V -> logic.
+
 Notation "r '↦ᵣ' v" :=
   (logic_assert_reg r v)
     (at level 70, no associativity, format "r ↦ᵣ v").
 
-Definition sProp_assert_reg (r : reg) (v : val) : sProp :=
-  fun ρ _ _ => get_reg r ρ = v.
 Instance assert_reg_single : LogicAssertReg reg val :=
-  sProp_assert_reg.
+  fun (r: reg) (v: val) ρ _ _ => get_reg r ρ = v.
 
-Definition sProp_assert_regs (rs : list reg) (vs : list val) : sProp :=
-  fun ρ _ _ => get_regs rs ρ = vs.
 Instance assert_reg_list : LogicAssertReg (list reg) (list val) :=
-  sProp_assert_regs.
-
-Definition sProp_register_entails (P : sProp) : sProp :=
-  fun _ m n => ∀ ρ, P ρ m n.
-
-Notation "'⊢ᵨ' P" :=
-  (sProp_register_entails P)
-    (at level 99, right associativity) : logic_scope.
+  fun (r: list reg) (v: list val) ρ _ _ => get_regs r ρ = v.
 
 Create HintDb custom_anyProp discriminated.
 
 Hint Unfold
-  lift_oProp
+  (* lift_oProp *)
   logic_and
   logic_or
   logic_impl
@@ -180,23 +137,21 @@ Hint Unfold
   (* logic_entails *)
   logic_empty_entails
   logic_pure
+  logic_memory_pure
   logic_later
   logic_always
   logic_memory_entails
+  logic_register_entails
 
-  oProp_update
-  oProp_set
-  oProp_assert
+  logic_set_mem
+  logic_assert_mem
 
-  sProp_set_reg
-  sProp_assert_reg
-  sProp_assert_regs
+  logic_set_reg
+  logic_assert_reg
 
   logic_assert_reg
   assert_reg_single
   assert_reg_list
-
-  sProp_register_entails
 
 : custom_anyProp.
 
